{
 "cells": [
  {
   "cell_type": "markdown",
   "id": "2180cbb6",
   "metadata": {},
   "source": [
    "# Exponents \n",
    "\n",
    "## Fundamentals of Exponents\n",
    "$$\n",
    "  2^{3} = 8; base^{exponent}\n",
    "$$"
   ]
  },
  {
   "cell_type": "code",
   "execution_count": 1,
   "id": "160c0570",
   "metadata": {},
   "outputs": [
    {
     "name": "stdout",
     "output_type": "stream",
     "text": [
      "8\n"
     ]
    }
   ],
   "source": [
    "answer = 2**3\n",
    "print(answer)"
   ]
  },
  {
   "cell_type": "markdown",
   "id": "3f60d593",
   "metadata": {},
   "source": [
    "Exponential notation consists of two parts: the **base** and the **exponent**. The exponent shows how many times to multiply the base by itself. In this case, $2^3$ means multiplying 2 by itself three times: 2 √ó 2 √ó 2 = 8.\n",
    "\n",
    "```{note}\n",
    "When we say '_base to the power of n_,' we are referring to raising the base to an exponent.\n",
    "```\n",
    "\n",
    "##### Rules For Exponentation \n",
    "::::{grid}\n",
    ":gutter: 2\n",
    "\n",
    ":::{grid-item}\n",
    ":outline:\n",
    "**Product of Powers Rule**  \n",
    "$base^m * base^n = base^{m+n}$  \n",
    "When multiplying powers with the same base, add the exponents.\n",
    ":::\n",
    "\n",
    ":::{grid-item}\n",
    ":outline:\n",
    "**Quotient of Powers Rule**  \n",
    "$\\frac{base^m}{base^n} = base^{m-n}$  \n",
    "When dividing powers with the same base, subtract the exponents.\n",
    ":::\n",
    "\n",
    ":::{grid-item}\n",
    ":outline:\n",
    "**Power of a Power Rule**  \n",
    "$(base^m)^n = base^{m * n}$  \n",
    "When raising a power to another power, multiply the exponents.\n",
    ":::\n",
    "\n",
    ":::{grid-item}\n",
    ":outline:\n",
    "**Power of a Product Rule**  \n",
    "$(ab)^n = a^n * b^n$  \n",
    "When raising a product to a power, raise each factor to the power.\n",
    ":::\n",
    "\n",
    ":::{grid-item}\n",
    ":outline:\n",
    "**Power of a Quotient Rule**  \n",
    "$(\\frac{a}{b})^n = \\frac{a^n}{b^n}$  \n",
    "When raising a quotient to a power, raise both the numerator and denominator to the power.\n",
    ":::\n",
    "\n",
    ":::{grid-item}\n",
    ":outline:\n",
    "**Exponent of a Fraction Rule**  \n",
    "$a^{\\frac{exp}{root}} = \\sqrt[root]{a^{exp}}$ or $(\\sqrt[root]{a})^{exp}$  \n",
    "A fractional exponent represents both a root and a power.\n",
    ":::\n",
    ":::: \n",
    "\n",
    "##### Definitions For Exponentation \n",
    "(1) $base^0 = 1$<br>\n",
    "Proof: \n",
    "Lets say we have a case where $base^{n}$ * $base^{-n}$ => $base^{n}/base^{n}$ = 1, so by using\n",
    "the quotient of powers property we see the $base^{n - n = 0} = 1$\n",
    "\n",
    "(2) $base^1 = base$<br>\n",
    "\n",
    "(3) $base^n$ = $base_{1}$ * $base_{2}$ * .... * $base_{n}$<br> \n",
    "\n",
    "(4a) $base^{-1}$ = $1/base^{1}$<br>\n",
    "(4b) $base^{-n}$ = $1/base^{n}$<br>\n",
    "A base raised to a negative exponent is equivalent to the reciprocal of the base raised to the positive exponent. \n",
    "\n",
    "Proof:<br>\n",
    "$\n",
    "\\frac{base^n}{base^n} = base^{n-n} = base^0 = 1\n",
    "$\n",
    "Since $base^0 = 1$, we have:\n",
    "\n",
    "$\n",
    "base^{-n} = \\frac{base^0}{base^n} = \\frac{1}{base^n}\n",
    "$"
   ]
  },
  {
   "cell_type": "code",
   "execution_count": 2,
   "id": "52aa12ab",
   "metadata": {},
   "outputs": [
    {
     "name": "stdout",
     "output_type": "stream",
     "text": [
      "Rule (1) base^0 = 1\n",
      "Rule (2) base^1 = 5\n",
      "Rule (3) base^n = 125\n",
      "Rule (4a) base^-1 = 0.2\n",
      "Rule (4b) base^-3 = 0.008\n"
     ]
    }
   ],
   "source": [
    "base = 5\n",
    "\n",
    "base_0 = base ** 0\n",
    "print(f\"Rule (1) base^0 = {base_0}\")\n",
    "\n",
    "base_1 = base ** 1\n",
    "print(f\"Rule (2) base^1 = {base_1}\")\n",
    "\n",
    "n = 3\n",
    "base_n = base ** n\n",
    "print(f\"Rule (3) base^n = {base_n}\")\n",
    "\n",
    "base_neg_1 = base ** -1\n",
    "print(f\"Rule (4a) base^-1 = {base_neg_1}\")\n",
    "\n",
    "base_neg_n = base ** -n\n",
    "print(f\"Rule (4b) base^-{n} = {base_neg_n}\")"
   ]
  },
  {
   "cell_type": "markdown",
   "id": "ba5d727d",
   "metadata": {},
   "source": [
    "##### Definitions for Radicals\n",
    "A **radical** in mathematics is a symbol used to find the root of a number. It shows the operation of determining a number that, when raised to a certain power, equals the value under the radical.\n",
    "\n",
    "**Assuming a positive (x)**\n",
    "\n",
    "$\\sqrt[n]{x} = x^{\\frac{1}{n}}$\n",
    "<br>\n",
    "Example: \n",
    "$\\sqrt[3]{25} = 25^{\\frac{1}{3}} = 5$\n",
    "\n",
    "**Assuming a negative (x) and an odd numbered root:**\n",
    "\n",
    "$n = 2k + 1 \\quad \\text{for some} \\, k \\in \\mathbb{Z}.$\n",
    "When we write ùëò ‚àà ùëç , we are saying that ùëò is an integer, i.e., it can be any of the numbers in the set ùëç. Therefore, ùëò could be any positive integer, negative integer, or zero.\n",
    "\n",
    "$\\sqrt[n]{x} = x^{\\frac{1}{n}}$\n",
    "<br>\n",
    "Example: \n",
    "$\\sqrt[3]{-8} = -8^{\\frac{1}{3}} = -2$\n",
    "\n",
    "**Assuming a negative (x) and an even numbered root:**\n",
    "\n",
    "$n = 2k \\quad \\text{for some} \\, k \\in \\mathbb{Z}.$\n",
    "\n",
    "Example: \n",
    "$\\sqrt[2]{-8} = -8^{\\frac{1}{2}} = ?$ (not a real number)\n",
    "\n",
    "##### Definitions for Fractional Exponents\n",
    "The root of a product is the product of the roots:<br>\n",
    "$(xy)^{\\frac{1}{n}} = \\sqrt[n]{x} * \\sqrt[n]{y} = \\sqrt[n]{xy}$\n",
    "\n",
    "The root of a quotient is the quotient of the roots:<br>\n",
    "$(\\frac{x}{y})^{\\frac{1}{n}} = \\frac{\\sqrt[n]{x}}{\\sqrt[n]{y}} = \\sqrt[n]{\\frac{x}{y}}$\n",
    "\n",
    "##### Practice Problems\n",
    "\n",
    "(1) Simplify: $3x(2x)^{3}(x^{-1})$\n",
    "\n",
    "```{dropdown} Answer\n",
    "  $3x^{1}(2)^{3}(x)^{3}\\left(\\frac{1}{x^{1}}\\right) = 8(3x)(x^{3})\\left(\\frac{1}{x^{1}}\\right) = 8(3x)x^{3-1} = 24x(x^{2}) = 24x^{3}$\n",
    "```\n",
    "\n",
    "(2) Simplify: $(\\frac{2^{-3}}{L})^{-2}$\n",
    "\n",
    "```{dropdown} Answer\n",
    "  $\\frac{2^{-3*-2}}{L^{-2}}$ = $\\frac{2^{6}}{\\frac{1}{L^{2}}}$ = $2^{6}L^{2}$ = $64L^{2}$\n",
    "```\n",
    "\n",
    "(3) Simplify: $\\frac{y^{4}(x^{6}y^{2})^{-2}}{(2x^{-3}y^{4})^{2}}$\n",
    "\n",
    "```{dropdown} Answer\n",
    "  $\\frac{y^{4}(x^{-12}y^{-4})}{(2^{2}x^{-6}y^{8})}$ = $\\frac{y^{4+(-4)}x^{-12}}{(4x^{-6}y^{8})}$ = $\\frac{x^{-12-(-6)}}{(4y^{8})}$ = $\\frac{x^{-6}}{4y^{8}}$ = $x^{-6} * \\frac{1}{4y^{8}}$ = $x^{-6} * y^{-8} * \\frac{1}{4}$\n",
    "```\n",
    "\n",
    "(4) Solve: $27^{\\frac{2}{3}}$\n",
    "\n",
    "```{dropdown} Answer\n",
    "  $\\sqrt[3]{27^{2}} or (\\sqrt[3]{27})^{2} = 3^{2} = 9$\n",
    "```\n",
    "\n",
    "(5) Solve: $\\frac{x^\\frac{-2}{3}\\sqrt[2]{x}y^{-2}{3}}{x^{\\frac{3}{2}}\\sqrt[3]{y}}$\n",
    "\n",
    "```{dropdown} Answer\n",
    "  $x^{\\frac{-2}{3} + \\frac{1}{2} - \\frac{3}{2}} * y^{\\frac{-2}{3} - \\frac{1}{3}} = x^{\\frac{-10}{6}} * y^{-1}$ \n",
    "```"
   ]
  },
  {
   "cell_type": "code",
   "execution_count": 3,
   "id": "db83c24b",
   "metadata": {},
   "outputs": [
    {
     "name": "stdout",
     "output_type": "stream",
     "text": [
      "Expression 1:\n",
      "     3\n",
      "24‚ãÖx \n",
      "Expression 2:\n",
      "       2\n",
      "64.0‚ãÖL \n",
      "Expression 3:\n",
      "    1   \n",
      "‚îÄ‚îÄ‚îÄ‚îÄ‚îÄ‚îÄ‚îÄ\n",
      "   6  8\n",
      "4‚ãÖx ‚ãÖy \n",
      "Expression 4:\n",
      " 9.00000000000000\n",
      "Expression 5:\n",
      "  -1.66666666666667  -1.0\n",
      "x                 ‚ãÖy    \n"
     ]
    }
   ],
   "source": [
    "from sympy import symbols, simplify, Eq\n",
    "from sympy.printing import pretty\n",
    "\n",
    "x, y, L = symbols('x y L')\n",
    "\n",
    "expr1 = 3 * x * (2 * x)**3 * x**(-1)\n",
    "expr2 = (2**(-3) / L)**(-2)\n",
    "expr3 = (y**4 * (x**6 * y**2)**(-2)) / ((2 * x**(-3) * y**4)**2)\n",
    "expr4 = 27**(2/3)\n",
    "expr5 = (x**(-2/3) * (x**(1/2)) * y**(-2/3)) / (x**(3/2) * y**(1/3))\n",
    "\n",
    "simplified_expr1 = simplify(expr1)\n",
    "simplified_expr2 = simplify(expr2)\n",
    "simplified_expr3 = simplify(expr3)\n",
    "simplified_expr4 = simplify(expr4)\n",
    "simplified_expr5 = simplify(expr5)\n",
    "\n",
    "print(\"Expression 1:\\n\", pretty(simplified_expr1))\n",
    "print(\"Expression 2:\\n\", pretty(simplified_expr2))\n",
    "print(\"Expression 3:\\n\", pretty(simplified_expr3))\n",
    "print(\"Expression 4:\\n\", pretty(simplified_expr4))\n",
    "print(\"Expression 5:\\n\", pretty(simplified_expr5))"
   ]
  }
 ],
 "metadata": {
  "jupytext": {
   "formats": "md:myst",
   "text_representation": {
    "extension": ".md",
    "format_name": "myst",
    "format_version": 0.13,
    "jupytext_version": "1.11.5"
   }
  },
  "kernelspec": {
   "display_name": "Python 3",
   "language": "python",
   "name": "python3"
  },
  "language_info": {
   "codemirror_mode": {
    "name": "ipython",
    "version": 3
   },
   "file_extension": ".py",
   "mimetype": "text/x-python",
   "name": "python",
   "nbconvert_exporter": "python",
   "pygments_lexer": "ipython3",
   "version": "3.10.7"
  },
  "source_map": [
   13,
   21,
   24,
   103,
   121,
   189
  ]
 },
 "nbformat": 4,
 "nbformat_minor": 5
}